Day 3

problems/3/Problem3.dfy
@@ -1,9 +1,79 @@
+include "../../parser/split.dfy"
+include "../../parser/parseInt.dfy"
 module Problem3 {
+    import opened Split
+    import opened ParseInt
+    import opened Std.Collections.Seq
+
+    method parseInput(input: string) returns (xs: seq<seq<nat>>) {
+        var lines := splitOnBreak(input);
+        xs := [];
+        for i := 0 to |lines| 
+            invariant |xs| == i
+        {
+            var bank := Map(Integer, split(lines[i],""));
+            expect forall i :: 0 <= i < |bank| ==> bank[i] > 0;
+            xs := xs + [bank];
+        }
+    }
+
+    function ToNat(bank: seq<nat>): nat {
+        if bank == [] then 0
+        else bank[|bank|-1] + 10*ToNat(bank[..|bank|-1])
+    }
+
+    function MaxIndex(xs: seq<nat>): (nat, nat)
+        requires |xs| > 0
+        ensures 0 <= MaxIndex(xs).1 < |xs|
+        ensures MaxIndex(xs).0 == xs[MaxIndex(xs).1]
+        ensures forall i :: 0 <= i < |xs| ==> MaxIndex(xs).0 >= xs[i]
+    {
+        if |xs| == 1 then
+            (xs[0], 0)
+        else
+            var rest := MaxIndex(xs[1..]);
+            if xs[0] >= rest.0 then
+                (xs[0], 0)
+            else
+                assert xs == [xs[0]]+xs[1..];
+                (rest.0, rest.1+1)
+    }
+
+    function fls(xs: seq<nat>, index: nat, count: nat): seq<nat>
+        requires |xs| > count
+        requires index < |xs|-count+1
+        requires count > 0
+        decreases count
+        ensures |fls(xs, index, count)| == count
+    {
+       if count == 1 then
+         var mi := MaxIndex(xs[index..]);
+         [mi.0]
+       else
+         var mi := MaxIndex(xs[index..|xs|-count+1]);
+         [mi.0]+fls(xs, index+mi.1+1, count-1)
+    }
+    
     method problem3_1(input: string) returns (x: int) {
-        return 3;
+        var banks := parseInput(input);
+        x := 0;
+        for i := 0 to |banks|
+        {
+            expect |banks[i]| > 2;
+            var best := fls(banks[i], 0, 2);
+            x := x + ToNat(best);
+        }
     }
 
     method problem3_2(input: string) returns (x: int) {
-        return 4;
+        var banks := parseInput(input);
+        x := 0;
+        for i := 0 to |banks|
+        {
+            expect |banks[i]| > 12;
+            var best := fls(banks[i], 0, 12);
+            x := x + ToNat(best);
+        }
+        print "\n";
     }
 }
